progess with NP proofs, attempts at reduction

theories/L/Complexity/Problems/Clique.v
@@ -1,10 +1,8 @@
 From Undecidability.L Require Import L.
 From Undecidability.L.Tactics Require Import LTactics ComputableTactics.
 From Undecidability.L.Datatypes Require Import LProd LTerm LNat Lists LOptions.
-From Undecidability.L.Complexity Require Import NP Synthetic Monotonic LinTimeDecodable. 
+From Undecidability.L.Complexity Require Import NP Synthetic Monotonic LinTimeDecodable Tactics Problems.LGraph.
 From Undecidability.L.Functions Require Import Size.
-
-From Undecidability.L.Datatypes Require Export LGraph. 
 
 
 (* k-Clique: duplicate-free list of k nodes such that all pairwise-distinct nodes are connected *)
@@ -27,7 +25,7 @@ Definition LClique (input : Lgraph * nat) :=
 Definition LClique_verifier (input : Lgraph * nat) (cert : term) :=
   let (g, k) := input in 
   exists (l : list nat),
-    cert = enc l /\ isLClique g l k. (*this includes that l is short enough*)
+     Some l = decode (list nat) cert /\ isLClique g l k. (*this includes that l is short enough*)
 
 Lemma isLClique_node_in (g : Lgraph) (k : nat) (cl : list Lnode) : isLClique g cl k -> forall n, n el cl -> Lgraph_node_in_dec g n = true. 
 Proof.
@@ -45,37 +43,6 @@ Lemma size_nat_enc_mono (n  :nat) (m : nat) :
 Proof. 
   intros H; repeat rewrite size_nat_enc. lia. 
 Qed. 
-
-Section dupfree_dec.
-  Variable (X : Type).
-  Variable (eqbX : X -> X -> bool).
-  Variable (eqbX_correct : forall a b, a = b <-> eqbX a b = true). 
-
-  Fixpoint dupfreeb (l : list X) : bool :=
-    match l with [] => true
-            | (x :: ls) => negb (list_in_decb eqbX ls x) && dupfreeb ls
-  end. 
-
-  Lemma dupfreeb_correct (l : list X) : reflect (dupfree l) (dupfreeb l).
-  Proof.
-    destruct dupfreeb eqn:H; constructor. 
-    - induction l; constructor. all: cbn in H; apply andb_prop in H. 
-      all: cbn in H; destruct H. apply ssrbool.negbTE in H.
-      now intros H1%(list_in_decb_iff eqbX_correct).
-      now apply IHl.  
-    - intros H0. induction H0. cbn in H; congruence. 
-      apply IHdupfree. cbn in H; apply andb_false_elim in H. destruct H.
-      apply ssrbool.negbFE in e. apply (list_in_decb_iff eqbX_correct) in e. tauto. 
-      assumption. 
-  Qed.
-
-  Lemma dupfreeb_iff (l : list X) : dupfreeb l = true <-> dupfree l. 
-  Proof. 
-    specialize (dupfreeb_correct l) as H0.
-    destruct dupfreeb. inv H0. split; eauto. inv H0; split; eauto. 
-  Qed.
-
-End dupfree_dec. 
 
 Fixpoint connectedb (g : Lgraph) (cl : list Lnode) :=
   match cl with [] => true
@@ -110,20 +77,6 @@ Definition LClique_verifierb (g : Lgraph) (k : nat) (cl : list Lnode) :=
 
 Definition nat_eqb_correct := (fun a b => conj (proj2 (Nat.eqb_eq a b)) (proj1 (Nat.eqb_eq a b))). 
 
-Ltac simp_bool := repeat match goal with
-                  | [ H: negb (?b) = true , H' : ?b = true |- _] => rewrite negb_true_iff in H; congruence
-                  | [H : negb (?b) = false |- _] => apply ssrbool.negbFE in H; unfold is_true in H
-                  | [H : negb (?b) = true |- _] => apply ssrbool.negbTE in H
-                  | [ H : andb (?b1) (?b2) = true |- _] => apply andb_prop in H;
-                                                         let a := fresh "H" in
-                                                         let b := fresh "H" in
-                                                         destruct H as [a b]
-                  | [H : andb (?b1) (?b2) = false |- _] => apply andb_false_elim in H;
-                                                         destruct H as [H | H]
-                  | [H : false = andb (?b1) (?b2) |- _] => symmetry in H; simp_bool
-                  | [ |- context[andb (?b1) (?b2) = false]] => rewrite andb_false_iff 
-                  end; try congruence.
-
 Lemma LClique_verifierb_correct (g : Lgraph) (k : nat) (cl : list Lnode) :
   reflect (isLClique g cl k) (LClique_verifierb g k cl). 
 Proof.
@@ -152,33 +105,9 @@ Proof.
       now apply H4 in H3.  
 Qed. 
 
+From Undecidability.L.Complexity Require Import PolyBounds ONotation Monotonic. 
 
 (*extraction of needed functions and derivation of runtime bounds in terms of encoding size*)
-
-Fixpoint dupfreeb_time (X : Type) (eqbT : X -> unit -> (nat * (X -> unit -> nat * unit ))) (l : list X) := match l with [] => 8 | l :: ls => list_in_decb_time eqbT ls l + 25 + dupfreeb_time eqbT ls end.
-Instance term_dupfreeb (X : Type) `{registered X}: computableTime' (@dupfreeb X) (fun eqb eqbT => (8, fun l _ => (dupfreeb_time eqbT l, tt))).
-Proof.
-  extract. 
-  solverec. 
-Defined. 
-
-Lemma dupfreeb_time_bound (X : Type) `{registered X} (eqbT : X -> unit -> (nat * (X -> unit -> nat * unit))):
-  (*eqbT is polynomial in encoding of a and b *)
-  (exists (f : nat -> nat), (forall (a b : X), callTime2 eqbT a b <= f (size(enc a) * size(enc b))) /\ inOPoly f)
-  -> exists (f : nat -> nat), (forall (l : list X), dupfreeb_time eqbT l <= f (size(enc l))) /\ inOPoly f. 
-Proof.
-  intros (f' & H1 & H2).  
-  evar (f : nat -> nat). exists f. split.
-  - intros l. unfold dupfreeb_time.  
-
-Definition forallb_time (X:Type) (fT : X -> unit -> nat * unit) (l : list X) := fold_right (fun elm acc => fst(fT elm tt) + acc + 15) 8 l.
-
-Instance term_forallb (X : Type) `{registered X} : computableTime' (@forallb X) (fun f fT => (1, fun l _ => (forallb_time fT l, tt))). 
-Proof.
-  extract. 
-  solverec. 
-  unfold forallb_time. solverec. 
-Defined. 
 
   Fixpoint connectedb_time (g : Lgraph) (cl : list Lnode) :=
     let (n, e) := g in 
@@ -195,54 +124,90 @@ Proof.
   solverec. 
 Qed. 
 
+Lemma connectedb_time_bound : exists (f : nat -> nat), (forall (g : Lgraph) (cl : list Lnode), connectedb_time g cl <= f (size(enc g) + size(enc cl))) /\ inOPoly f /\ monotonic f.
+Proof.
+  pose (forallb_step_t := fun (e : list Ledge) (cl_check : nat) => (fun (v : nat) (_ : unit) =>
+            (list_in_decb_time pair_eqb_nat_time e (cl_check, v) + list_in_decb_time pair_eqb_nat_time e (v, cl_check) + 29, tt))).
+  specialize (list_in_decb_time_bound pair_eqb_nat_time_bound) as (fin & H1 & H2 & H3). 
+  (* specialize (forallb_time_bound) *)
+  evar (f : nat -> nat). exists f. split.
+  - intros g cl. unfold connectedb_time.
+
+Admitted.  
+
 Definition Lclique_verifierb_time (g : Lgraph) (k:nat) (cl : list Lnode):= forallb_time (fun n _ => (33 + 14 * n, tt)) cl
   + dupfreeb_time (fun x _ => (5, fun y _ => (min x y * 17 + 9, tt))) cl
   + connectedb_time g cl + 11 * (|cl|) + 17 * min (|cl|) k + 53.
+
 Instance term_LClique_verifierb : computableTime' LClique_verifierb (fun g _ => (1, fun k _ => (1, fun cl _ => (Lclique_verifierb_time g k cl, tt)))). 
 Proof.
   extract. 
   solverec. unfold Lclique_verifierb_time. solverec. 
 Qed. 
+
+Lemma Lclique_verifierb_time_bound : exists (f : nat -> nat) , (forall (g: Lgraph) (k : nat) (cl : list Lnode), Lclique_verifierb_time g k cl <= f(size(enc g) + size(enc k) + size(enc cl))) /\ inOPoly f /\ monotonic f. 
+Proof.
+Admitted. 
                  
 Lemma clique_inNP : inNP LClique. 
 Proof.
   exists LClique_verifier. 
   3 : {
     intros [g k]; split.
-    - destruct g. intros (cert & H1). exists (enc cert), cert. split; try tauto.
+    - destruct g. intros (cert & H1). exists (enc cert), cert. split; try tauto. now rewrite decode_correct. 
     - intros (ter & cert & H1 & H2). now exists cert. 
   }
   2 : {
     evar (f' : nat -> nat). 
     exists f'. split. 2: split. 
     2: {
-      intros [g k] y (cert & H1 & H2).
-      assert (k = (|cert|)) by (now apply isLClique_length with (g:= g)).
-      rewrite H in *; clear H k. rewrite H1. rewrite size_prod; cbn [fst snd]. 
-      rewrite size_term_enc. rewrite size_nat_enc. rewrite size_list.   
-      recRel_prettify2.
-      (*LHS is in O(max_node * |cert|) *)
-      unfold Lgraph_node_in_dec in H2. destruct g.
-      assert (sumn (map (fun (x : nat ) => size (enc x) + 5) cert) <= (size(enc n) + 5) * (|cert|)). 
-      - clear H1. induction cert. cbn; lia.
-        cbn. assert (a <= n).
-        { assert (Lgraph_node_in_dec (n, l) a = true ).
-          apply isLClique_node_in with (k:= |a::cert|) (cl:= a::cert); easy.
-          cbn in H. destruct n. congruence. apply leb_complete in H. lia. 
-        } 
-        apply size_nat_enc_mono in H. rewrite H. rewrite IHcert. solverec. 
-        firstorder. now inv H2. 
-      - rewrite H. rewrite size_prod with (w := (n, l)); cbn [fst snd].
-        instantiate (f' := fun n => 4 * n * n). subst f'. 
-        solverec. 
-    }
-    all: (subst f'; smpl_inO). 
-  }
+      intros [g k] y (cert & H1 & H2). (*the missing injection problem, again*)
+Abort. 
+(*       assert (k = (|cert|)) by (now apply isLClique_length with (g:= g)). *)
+(*       rewrite H in *; clear H k. rewrite size_prod; cbn [fst snd].  *)
+(*       rewrite size_term_enc. rewrite size_nat_enc. rewrite size_list.    *)
+(*       recRel_prettify2. *)
+(*       (*LHS is in O(max_node * |cert|) *) *)
+(*       unfold Lgraph_node_in_dec in H2. destruct g. *)
+(*       assert (sumn (map (fun (x : nat ) => size (enc x) + 5) cert) <= (size(enc n) + 5) * (|cert|)).  *)
+(*       - clear H1. induction cert. cbn; lia. *)
+(*         cbn. assert (a <= n). *)
+(*         { assert (Lgraph_node_in_dec (n, l) a = true ). *)
+(*           apply isLClique_node_in with (k:= |a::cert|) (cl:= a::cert); easy. *)
+(*           cbn in H. destruct n. congruence. apply leb_complete in H. lia.  *)
+(*         }  *)
+(*         apply size_nat_enc_mono in H. rewrite H. rewrite IHcert. solverec.  *)
+(*         firstorder. now inv H2.  *)
+(*       - rewrite H. rewrite size_prod with (w := (n, l)); cbn [fst snd]. *)
+(*         instantiate (f' := fun n => 4 * n * n). subst f'.  *)
+(*         solverec.  *)
+(*     } *)
+(*     all: (subst f'; smpl_inO).  *)
+(*   } *)
 
-  evar (f : nat -> nat). exists f. split; try split. 
-  - exists (fun inp => match inp with ((g, k), cert) => match decode (list nat) cert with Some cert => LClique_verifierb g k cert | _ => false end end).
-    split.
-    + constructor. extract. solverec.
-      repeat (rewrite size_prod; cbn [fst snd]).
-      unfold Lclique_verifierb_time. 
-Admitted. 
+(*   destruct (Lclique_verifierb_time_bound) as (f' & H1 & H2 & H3). *)
+(*   evar (f : nat -> nat). exists f. split; try split.  *)
+(*   - exists (fun inp => match inp with ((g, k), cert) => match decode (list nat) cert with Some cert => LClique_verifierb g k cert | _ => false end end). *)
+(*     split. *)
+(*     + constructor. extract. solverec. *)
+(*       repeat (rewrite size_prod; cbn [fst snd]). *)
+(*       rewrite H1. rewrite size_prod; cbn [fst snd]. *)
+(*       instantiate (f:= fun n => c__linDec(list nat) * n + f'(n) + 15). subst f. *)
+(*       cbn. unfold monotonic in H3. rewrite H3 at 1.   *)
+(*       2 : { *)
+(*         assert (size(enc a) + size(enc b1) + 4 + size(enc b0) + size(enc l) <= size(enc a) + size(enc b1) + 4 + size(enc b0) + 4+ size(enc b) + 4).  *)
+(*         2: apply H0. enough (size(enc l) <= size(enc b)) by lia.  *)
+(*         (* intuitively, this should be clear, since b is an encoding of l *) *)
+(*         (* but since decode isn't injective, this seems to be difficult to prove*) *)
+(*         (* one way would be to prove injectivity for this particular instance*) *)
+(*         admit. *)
+(*       } *)
+(*       rewrite size_term_enc_r. solverec.  *)
+(*       subst f. solverec. repeat rewrite size_prod; cbn [fst snd]. rewrite size_term_enc_r. solverec.   *)
+(*   + intros [[g k] b]. specialize (LClique_verifierb_correct g k) as H4.  split.  *)
+(*     * cbn. intros (l & F1 & F2). rewrite F1. rewrite decode_correct. *)
+(*       destruct (reflect_iff (isLClique g l k) (LClique_verifierb g k l) ) as (F3 & _). apply H4. *)
+(*       apply F3, F2.  *)
+(*     * intros H. cbn. destruct (decode (list nat) b) eqn:H5. 2: congruence. exists l. *)
+(*       (*same enc/dec problem*) *)
+(* Admitted.  *)
