theories/L/Complexity/Problems/kSAT.v
@@ -1,0 +1,42 @@
+From Undecidability.L Require Import L.
+From Undecidability.L.Tactics Require Import LTactics ComputableTactics.
+From Undecidability.L.Datatypes Require Import LProd LTerm LNat Lists LOptions.
+From Undecidability.L.Complexity Require Import NP Synthetic Monotonic.
+From Undecidability.L.Functions Require Import Size.
+
+From Undecidability.L.Complexity Require Export Problems.SAT Tactics.
+
+Inductive kCNF (k : nat) : cnf -> Prop :=
+| kCNFB : k > 0 -> kCNF k []
+| kCNFS (c : cnf) (cl : clause) : (|cl|) = k -> kCNF k c -> kCNF k (cl :: c).               
+
+Definition kSAT (k : nat) (c : cnf) : Prop := kCNF k c /\ exists (a : assgn), evalCnf a c = Some true. 
+
+Definition kCNF_decb_pred (k : nat) := (fun (cl : clause) => Nat.eqb k (|cl|)).
+Definition kCNF_decb (k : nat) (c : cnf) := leb 1 k && forallb (kCNF_decb_pred k) c. 
+
+Lemma kCNF_decb_correct (k : nat) (c : cnf) : kCNF_decb k c = true <-> (k > 0 /\ forall (cl : clause), cl el c -> (k = |cl|)). 
+Proof.
+  unfold kCNF_decb, kCNF_decb_pred. 
+  split.
+  - intros H; simp_bool. rewrite forallb_forall in H1. split.
+    apply leb_complete in H0; lia. intros. rewrite <- Nat.eqb_eq. now apply H1.  
+  - intros [H1 H2]. simp_bool; split. apply Nat.leb_le; lia. 
+    rewrite forallb_forall. intros. rewrite Nat.eqb_eq. now apply H2. 
+Qed. 
+
+Lemma kCNF_kge (k : nat) (c : cnf) : kCNF k c -> k > 0.
+Proof. induction 1; assumption. Qed.
+
+Instance term_kCNF_decb_pred : computableTime' kCNF_decb_pred (fun k _ => (1, fun cl _ => (11 * (|cl|) + 17 * min k (|cl|) + 23, tt))).  
+Proof.
+  extract. 
+  solverec. 
+Defined. 
+
+Instance term_kCNF_decb : computableTime' kCNF_decb (fun k _ => (1, fun c _ => (forallb_time (fun cl _ => (11 * (|cl|) + 17 * min k (|cl|) + 23, tt)) c + 36, tt))).
+Proof.
+  extract. 
+  solverec. 
+Qed. 
+  
