theories/L/Complexity/Reductions/TSAT_to_SAT.v
@@ -1,4 +1,0 @@
-From Undecidability.L.Complexity Require Import NP Synthetic Problems.SAT Problems.Clique. 
-From Undecidability.L Require Import Tactics.LTactics.
-From Undecidability.L.Complexity Require Import Problems.TSAT. 
-
