theories/L/Complexity/Reductions/kSAT_to_SAT.v
@@ -1,0 +1,63 @@
+From Undecidability.L.Complexity Require Import NP Synthetic Problems.SAT Problems.Clique. 
+From Undecidability.L Require Import Tactics.LTactics.
+From Undecidability.L.Complexity Require Import Problems.kSAT PolyBounds Tactics NP. 
+From Undecidability.L.Datatypes Require Import LBool LNat Lists LProd. 
+
+Lemma evalCnf_inv_true (c : cnf) (cl :clause) (a : assgn) : (evalCnf a (cl::c) = Some true) -> (evalCnf a c = Some true). 
+Admitted. 
+
+Lemma ksat_to_sat (k : nat): reducesPolyMO (kSAT k) SAT. 
+Proof. 
+  (*check if it is a kCNF. if so, the reduction the SAT instance is the identity. otherwise, return a negative SAT instance*)
+  exists (fun x => if kCNF_decb k x then x else [[(true, 0)]; [(false, 0)]] ). 
+  split.
+  - pose (predT := (fun (cl : list (bool * nat)) (_ : unit) => (11 * (| cl |) + 17 * Init.Nat.min k (| cl |) + 23, tt))). 
+    assert (exists (fPred : nat -> nat), (forall (a : list (bool * nat)), fst(predT a tt) <= fPred (size(enc a))) /\ inOPoly fPred /\ monotonic fPred). 
+    * evar (fPred : nat -> nat). exists fPred. split; try split. 
+        1: {
+          intros a. unfold predT. cbn [fst]. instantiate (fPred := fun n => 28 * n + 23). subst fPred. 
+          induction a. 
+          + cbn; lia. 
+          + cbn -[Nat.mul]. solverec. rewrite Nat.le_min_r. solverec. rewrite list_size_cons. rewrite list_size_length. 
+            solverec. 
+        }
+      all: subst fPred; smpl_inO.
+    * specialize (forallb_time_bound H) as (f' & H1 & H2 & H3).
+      evar (f : nat -> nat). exists f.
+      + constructor.  extract. solverec.
+        2: { fold predT. rewrite H1. instantiate (f := fun n => f' n + 53). subst f. lia. }
+        fold predT. rewrite H1. subst f; lia.
+      + subst f; smpl_inO. 
+      + subst f; smpl_inO. 
+      + (* now we need to prove that the output of the reduction is polynomial *)
+        evar (tf : nat -> nat). exists tf. split. 
+        1 : {
+          intros x. destruct (kCNF_decb k x).
+          Compute (size(enc [[(true, 0)]; [(false, 0)]])).
+          instantiate (tf := fun n => n + 55).
+          all: subst tf. 2 : replace (size(enc [[(true, 0)]; [(false, 0)]])) with 55. 1-2: lia. 
+          now cbv. 
+        }
+        split; subst tf; smpl_inO. 
+  - intros x. split.
+    + intros ( H1 & a & H2). destruct (kCNF_decb k x) eqn:H3. now exists a. clear H2. 
+      induction H1. 
+      * unfold kCNF_decb in H3; simp_bool. rewrite Nat.leb_nle in H3. lia. cbn in H3; congruence.
+      * specialize (kCNF_decb_correct k c) as H4.
+        cbn in H3. simp_bool.
+        -- unfold kCNF_decb_pred in H3. unfold kCNF_decb in H3. simp_bool. rewrite Nat.leb_nle in H3.
+           apply kCNF_kge in H1; lia. cbn in H3; simp_bool. unfold kCNF_decb_pred in H3. 
+           now apply beq_nat_false in H3. apply IHkCNF. unfold kCNF_decb. simp_bool; right; apply H3. 
+    + intros (a & H). destruct (kCNF_decb k x) eqn:H1. split. rewrite kCNF_decb_correct in H1. 
+      induction x; constructor.
+      * tauto. 
+      * symmetry. apply H1. now left. 
+      * apply IHx. split; try tauto. intros cl H2. apply H1. now right. now apply evalCnf_inv_true with (cl:= a0). 
+      * now exists a. 
+      * destruct a. now cbn in H. destruct b; cbn in H; congruence.
+Qed. 
+
+Lemma inNP_kSAT (k : nat) : inNP (kSAT k). 
+Proof.
+  (* apply red_inNP with (Q := SAT). *)
+Admitted. 
