theories/L/Datatypes/LNat.v
@@ -105,6 +105,7 @@ Proof.
 Qed.
 
 
+
 (* This is an example for an function in which the run-time of the fix itself is not constant (in add, the fix on the first argument always returns an function in ~5 steps)*)
 (* Instance termT_testId : computableTime' (fix f x := *)
 (*                                             match x with *)
